BPlusTree_Split.thy
@@ -1,6 +1,65 @@
 theory BPlusTree_Split
-  imports BPlusTree_Set
+imports BPlusTree
 begin
+
+subsection "Auxiliary functions"
+
+(* a version of split half that assures the left side to be non-empty *)
+fun split_half:: "_ list \<Rightarrow> _ list \<times> _ list" where
+  "split_half xs = (take ((length xs + 1) div 2) xs, drop ((length xs + 1) div 2) xs)"
+
+lemma split_half_conc: "split_half xs = (ls, rs) = (xs = ls@rs \<and> length ls = (length xs + 1) div 2)"
+  by force
+
+lemma drop_not_empty: "xs \<noteq> [] \<Longrightarrow> drop (length xs div 2) xs \<noteq> []"
+  apply(induction xs)
+   apply(auto split!: list.splits)
+  done
+
+lemma take_not_empty: "xs \<noteq> [] \<Longrightarrow> take ((length xs + 1) div 2) xs \<noteq> []"
+  apply(induction xs)
+   apply(auto split!: list.splits)
+  done
+
+lemma split_half_not_empty: "length xs \<ge> 1 \<Longrightarrow> \<exists>ls a rs. split_half xs = (ls@[a],rs)"
+  using take_not_empty
+  by (metis (no_types, hide_lams) Ex_list_of_length One_nat_def le_trans length_Cons list.size(4) nat_1_add_1 not_one_le_zero rev_exhaust split_half.simps take0 take_all_iff)
+
+subsection "The split function locale"
+
+text "Here, we abstract away the inner workings of the split function
+      for B-tree operations."
+
+locale split_tree =
+  fixes split ::  "('a bplustree\<times>'a::{linorder,order_top}) list \<Rightarrow> 'a \<Rightarrow> (('a bplustree\<times>'a) list \<times> ('a bplustree\<times>'a) list)"
+  assumes split_req:
+    "\<lbrakk>split xs p = (ls,rs)\<rbrakk> \<Longrightarrow> xs = ls @ rs"
+    "\<lbrakk>split xs p = (ls@[(sub,sep)],rs); sorted_less (separators xs)\<rbrakk> \<Longrightarrow> sep < p"
+    "\<lbrakk>split xs p = (ls,(sub,sep)#rs); sorted_less (separators xs)\<rbrakk> \<Longrightarrow> p \<le> sep"
+begin
+  lemmas split_conc = split_req(1)
+  lemmas split_sorted = split_req(2,3)
+  
+  
+  lemma [termination_simp]:"(ls, (sub, sep) # rs) = split ts y \<Longrightarrow>
+        size sub < Suc (size_list (\<lambda>x. Suc (size (fst x))) ts  + size l)"
+    using split_conc[of ts y ls "(sub,sep)#rs"] by auto
+end
+
+locale split_list =
+  fixes split_list ::  "('a::{linorder,order_top}) list \<Rightarrow> 'a \<Rightarrow> 'a list \<times> 'a list"
+  assumes split_list_req:
+    "\<lbrakk>split_list ks p = (kls,krs)\<rbrakk> \<Longrightarrow> ks = kls @ krs"
+    "\<lbrakk>split_list ks p = (kls@[sep],krs); sorted_less ks\<rbrakk> \<Longrightarrow> sep < p"
+    "\<lbrakk>split_list ks p = (kls,(sep)#krs); sorted_less ks\<rbrakk> \<Longrightarrow> p \<le> sep"
+
+locale split_full = split_tree: split_tree split + split_list split_list
+    for split::
+      "('a bplustree \<times> 'a::{linorder,order_top}) list \<Rightarrow> 'a
+         \<Rightarrow> ('a bplustree \<times> 'a) list \<times> ('a bplustree \<times> 'a) list"
+    and split_list::
+      "'a::{linorder,order_top} list \<Rightarrow> 'a
+         \<Rightarrow> 'a list \<times> 'a list"
 
 section "Abstract split functions"
 
@@ -13,10 +72,7 @@ text "Linear split is similar to well known functions, therefore a quick proof c
 fun linear_split where "linear_split xs x = (takeWhile (\<lambda>(_,s). s<x) xs, dropWhile (\<lambda>(_,s). s<x) xs)"
 fun linear_split_list where "linear_split_list xs x = (takeWhile (\<lambda>s. s<x) xs, dropWhile (\<lambda>s. s<x) xs)"
 
-global_interpretation bplustree_linear_search_list: split_list linear_split_list
-  defines bplustree_ls_isin_list = bplustree_linear_search_list.isin_list 
-    and bplustree_ls_insert_list = bplustree_linear_search_list.insert_list
-    and bplustree_ls_delete_list = bplustree_linear_search_list.delete_list
+interpretation bplustree_linear_search_list: split_list linear_split_list
   apply unfold_locales
   unfolding linear_split.simps
     apply (auto split: list.splits)
@@ -26,114 +82,14 @@ global_interpretation bplustree_linear_search_list: split_list linear_split_list
     by (metis case_prod_conv hd_dropWhile le_less_linear list.sel(1) list.simps(3))
   done
 
-global_interpretation bplustree_linear_search:
-    split_set linear_split bplustree_ls_isin_list bplustree_ls_insert_list bplustree_ls_delete_list
-  (* the below definitions are required to be set here for evaluating example code... *)
-  defines bplustree_ls_isin = bplustree_linear_search.isin 
-    and bplustree_ls_ins = bplustree_linear_search.ins
-    and bplustree_ls_insert = bplustree_linear_search.insert
-    and bplustree_ls_del = bplustree_linear_search.del
-    and bplustree_ls_delete = bplustree_linear_search.delete
+interpretation bplustree_linear_search: split_tree linear_split
   apply unfold_locales
   unfolding linear_split.simps
-  subgoal by (auto split: list.splits)
-  subgoal
     apply (auto split: list.splits)
+  subgoal
     by (metis (no_types, lifting) case_prodD in_set_conv_decomp takeWhile_eq_all_conv takeWhile_idem)
-  subgoal by (metis case_prod_conv hd_dropWhile le_less_linear list.sel(1) list.simps(3))
-  subgoal using bplustree_linear_search_list.isin_list_set by blast
-  subgoal using bplustree_linear_search_list.insert_list_set by blast
-  subgoal using bplustree_linear_search_list.delete_list_set by blast
+  subgoal
+    by (metis case_prod_conv hd_dropWhile le_less_linear list.sel(1) list.simps(3))
   done
-
-
-text "Some examples follow to show that the implementation works
-      and the above lemmas make sense. The examples are visualized in the thesis."
-
-abbreviation "bplustree\<^sub>q \<equiv> bplustree_ls_isin"
-abbreviation "bplustree\<^sub>i \<equiv> bplustree_ls_insert"
-abbreviation "bplustree\<^sub>d \<equiv> bplustree_ls_delete"
-
-definition "uint8_max \<equiv> 2^8-1::nat"
-declare uint8_max_def[simp]
-
-typedef uint8 = "{n::nat. n \<le> uint8_max}" 
-  by auto
-
-setup_lifting type_definition_uint8
-
-instantiation uint8 :: linorder
-begin
-
-lift_definition less_eq_uint8 :: "uint8 \<Rightarrow> uint8 \<Rightarrow> bool"
-  is "(less_eq::nat \<Rightarrow> nat \<Rightarrow> bool)" .
-
-lift_definition less_uint8 :: "uint8 \<Rightarrow> uint8 \<Rightarrow> bool"
-  is "(less::nat \<Rightarrow> nat \<Rightarrow> bool)" .
-
-instance
-  by standard (transfer; auto)+
-end
-
-instantiation uint8 :: order_top
-begin
-
-lift_definition top_uint8 :: uint8 is "uint8_max::nat"
-  by simp
-
-
-instance 
-  by standard (transfer; simp)
-end
-
-
-instantiation uint8 :: numeral
-begin
-
-lift_definition one_uint8 :: uint8 is "1::nat"
-  by auto
-
-lift_definition plus_uint8 :: "uint8 \<Rightarrow> uint8 \<Rightarrow> uint8"
-  is "\<lambda>a b. min (a + b) uint8_max"
-  by simp
-
-instance by standard (transfer; auto)
-end
-
-instantiation uint8 :: equal
-begin
-
-lift_definition equal_uint8 :: "uint8 \<Rightarrow> uint8 \<Rightarrow> bool"
-  is "(=)" .
-
-instance by standard (transfer; auto)
-end
-
-
-value "uint8_max"
-
-value "let k=2::nat; x::uint8 bplustree = (Node [(Node [(LNode [1,2], 2),(LNode [3,4], 4),(LNode [5,6,7], 8)] (LNode [9,10]), 10)] (Node [(LNode [11,12,13,14], 14), (LNode [15,17], 20)] (LNode [21,22,23]))) in
-      root_order k x"
-value "let k=2::nat; x::uint8 bplustree = (Node [(Node [(LNode [1,2], 2),(LNode [3,4], 4),(LNode [5,6,7], 8)] (LNode [9,10]), 10)] (Node [(LNode [11,12,13,14], 14), (LNode [15,17], 20)] (LNode [21,22,23]))) in
-      bal x"
-value "let k=2::nat; x::uint8 bplustree = (Node [(Node [(LNode [1,2], 2),(LNode [3,4], 4),(LNode [5,6,7], 8)] (LNode [9,10]), 10)] (Node [(LNode [11,12,13,14], 14), (LNode [15,17], 20)] (LNode [50,55,56]))) in
-      sorted_less (leaves x)"
-value "let k=2::nat; x::uint8 bplustree = (Node [(Node [(LNode [1,2], 2),(LNode [3,4], 4),(LNode [5,6,7], 8)] (LNode [9,10]), 10)] (Node [(LNode [11,12,13,14], 14), (LNode [15,17], 20)] (LNode [50,55,56]))) in
-      Laligned x top"
-value "let k=2::nat; x::uint8 bplustree = (Node [(Node [(LNode [1,2], 2),(LNode [3,4], 4),(LNode [5,6,7], 8)] (LNode [9,10]), 10)] (Node [(LNode [11,12,13,14], 14), (LNode [15,17], 20)] (LNode [50,55,56]))) in
-      x"
-value "let k=2::nat; x::uint8 bplustree = (Node [(Node [(LNode [1,2], 2),(LNode [3,4], 4),(LNode [5,6,7], 8)] (LNode [9,10]), 10)] (Node [(LNode [11,12,13,14], 14), (LNode [15,17], 20)] (LNode [50,55,56]))) in
-      bplustree\<^sub>q x 4"
-value "let k=2::nat; x::uint8 bplustree = (Node [(Node [(LNode [1,2], 2),(LNode [3,4], 4),(LNode [5,6,7], 8)] (LNode [9,10]), 10)] (Node [(LNode [11,12,13,14], 14), (LNode [15,17], 20)] (LNode [50,55,56]))) in
-      bplustree\<^sub>q x 20"
-value "let k=2::nat; x::uint8 bplustree = (Node [(Node [(LNode [1,2], 2),(LNode [3,4], 4),(LNode [5,6,7], 8)] (LNode [9,10]), 10)] (Node [(LNode [11,12,13,14], 14), (LNode [15,17], 20)] (LNode [50,55,56]))) in
-      bplustree\<^sub>i k 9 x"
-value "let k=2::nat; x::uint8 bplustree = (Node [(Node [(LNode [1,2], 2),(LNode [3,4], 4),(LNode [5,6,7], 8)] (LNode [9,10]), 10)] (Node [(LNode [11,12,13,14], 14), (LNode [15,17], 20)] (LNode [50,55,56]))) in
-      bplustree\<^sub>i k 1 (bplustree\<^sub>i k 9 x)"
-value "let k=2::nat; x::uint8 bplustree = (Node [(Node [(LNode [1,2], 2),(LNode [3,4], 4),(LNode [5,6,7], 8)] (LNode [9,10]), 10)] (Node [(LNode [11,12,13,14], 14), (LNode [15,17], 20)] (LNode [50,55,56]))) in
-      bplustree\<^sub>d k 10 (bplustree\<^sub>i k 1 (bplustree\<^sub>i k 9 x))"
-value "let k=2::nat; x::uint8 bplustree = (Node [(Node [(LNode [1,2], 2),(LNode [3,4], 4),(LNode [5,6,7], 8)] (LNode [9,10]), 10)] (Node [(LNode [11,12,13,14], 14), (LNode [15,17], 20)] (LNode [50,55,56]))) in
-      bplustree\<^sub>d k 3 (bplustree\<^sub>d k 10 (bplustree\<^sub>i k 1 (bplustree\<^sub>i k 9 x)))"
-
 
 end
